rocq-brick-libstdcpp/proof/cstring/spec.v
@@ -10,6 +10,15 @@ Require Import skylabs.brick.libstdcpp.cstring.inc_cstring_cpp.
 
 #[local] Set Primitive Projections.
 
+#[local] Open Scope Z_scope.
+
+Notation search_result p found :=
+  match found with
+  | Some 0 => Vptr p
+  | Some off => Vptr (p .[ Tchar ! off ])
+  | None => Vptr nullptr
+  end (only parsing).
+
 Section with_cpp.
   Context `{Σ : cpp_logic, module ⊧ σ}.
 
@@ -33,4 +42,76 @@ Section with_cpp.
      \prepost{q1 s1} s1_p |-> cstring.R q1 s1
      \prepost{q2 s2} s2_p |-> cstring.R q2 s2
      \post[Vint (strncmp s1 s2 n)] emp).
+
+  cpp.spec "strchr(char*, int)" as strchr_mut_spec with
+    (\arg{s_p} "__s" (Vptr s_p)
+     \arg{c} "__c" (Vint c)
+     \prepost{q s} s_p |-> cstring.R q s
+     \require valid<"unsigned char"> c
+     \post[search_result s_p (strchr s c)] emp).
+
+  cpp.spec "strchr(const char*, int)" as strchr_const_spec with
+    (\arg{s_p} "__s" (Vptr s_p)
+     \arg{c} "__c" (Vint c)
+     \prepost{q s} s_p |-> cstring.R q s
+     \require valid<"unsigned char"> c
+     \post[search_result s_p (strchr s c)] emp).
+
+  cpp.spec "strrchr(char*, int)" as strrchr_mut_spec with
+    (\arg{s_p} "__s" (Vptr s_p)
+     \arg{c} "__c" (Vint c)
+     \prepost{q s} s_p |-> cstring.R q s
+     \require valid<"unsigned char"> c
+     \post[search_result s_p (strrchr s c)] emp).
+
+  cpp.spec "strrchr(const char*, int)" as strrchr_const_spec with
+    (\arg{s_p} "__s" (Vptr s_p)
+     \arg{c} "__c" (Vint c)
+     \prepost{q s} s_p |-> cstring.R q s
+     \require valid<"unsigned char"> c
+     \post[search_result s_p (strrchr s c)] emp).
+
+  cpp.spec "strspn" with
+    (\arg{s_p} "__s" (Vptr s_p)
+     \arg{accept_p} "__accept" (Vptr accept_p)
+     \prepost{q s} s_p |-> cstring.R q s
+     \prepost{accept_q accept} accept_p |-> cstring.R accept_q accept
+     \require valid<"unsigned long"> (strspn s accept)
+     \post[Vn (strspn s accept)] emp).
+
+  cpp.spec "strcspn" with
+    (\arg{s_p} "__s" (Vptr s_p)
+     \arg{reject_p} "__reject" (Vptr reject_p)
+     \prepost{q s} s_p |-> cstring.R q s
+     \prepost{reject_q reject} reject_p |-> cstring.R reject_q reject
+     \require valid<"unsigned long"> (strcspn s reject)
+     \post[Vn (strcspn s reject)] emp).
+
+  cpp.spec "strpbrk(char*, const char*)" as strpbrk_mut_spec with
+    (\arg{s_p} "__s" (Vptr s_p)
+     \arg{accept_p} "__accept" (Vptr accept_p)
+     \prepost{q s} s_p |-> cstring.R q s
+     \prepost{accept_q accept} accept_p |-> cstring.R accept_q accept
+     \post[search_result s_p (strpbrk s accept)] emp).
+
+  cpp.spec "strpbrk(const char*, const char*)" as strpbrk_const_spec with
+    (\arg{s_p} "__s" (Vptr s_p)
+     \arg{accept_p} "__accept" (Vptr accept_p)
+     \prepost{q s} s_p |-> cstring.R q s
+     \prepost{accept_q accept} accept_p |-> cstring.R accept_q accept
+     \post[search_result s_p (strpbrk s accept)] emp).
+
+  cpp.spec "strstr(char*, const char*)" as strstr_mut_spec with
+    (\arg{haystack_p} "__haystack" (Vptr haystack_p)
+     \arg{needle_p} "__needle" (Vptr needle_p)
+     \prepost{haystack_q haystack} haystack_p |-> cstring.R haystack_q haystack
+     \prepost{needle_q needle} needle_p |-> cstring.R needle_q needle
+     \post[search_result haystack_p (strstr haystack needle)] emp).
+
+  cpp.spec "strstr(const char*, const char*)" as strstr_const_spec with
+    (\arg{haystack_p} "__haystack" (Vptr haystack_p)
+     \arg{needle_p} "__needle" (Vptr needle_p)
+     \prepost{haystack_q haystack} haystack_p |-> cstring.R haystack_q haystack
+     \prepost{needle_q needle} needle_p |-> cstring.R needle_q needle
+     \post[search_result haystack_p (strstr haystack needle)] emp).
 End with_cpp.
